Exposed group notations and replaced Definition commands with Theorem commands, where appropriate, in group.v

group.v
@@ -127,7 +127,9 @@ Definition op_is_id_r := Monoid.op_is_id_r op_monoid.
 Definition op_is_id := Monoid.op_is_id op_monoid.
 
 (** Proves that 0 is the identity element. *)
-Definition op_id := Monoid.op_id op_monoid.
+Theorem op_id
+  :  op_is_id 0.
+Proof Monoid.op_id op_monoid.
 
 (**
   Accepts two group elements, x and y, and
@@ -142,29 +144,29 @@ Definition op_is_inv_l := Monoid.op_is_inv_l op_monoid.
 Definition op_is_inv_r := Monoid.op_is_inv_r op_monoid.
 
 (** Proves that the left identity element is unique. *)
-Definition op_id_l_uniq
-  :  forall x : E, (op_is_id_l x) -> x = 0
-  := Monoid.op_id_l_uniq op_monoid.
+Theorem op_id_l_uniq
+  :  forall x : E, (op_is_id_l x) -> x = 0.
+Proof Monoid.op_id_l_uniq op_monoid.
 
 (** Proves that the right identity element is unique. *)
-Definition op_id_r_uniq 
-  :  forall x : E, (op_is_id_r x) -> x = 0
-  := Monoid.op_id_r_uniq op_monoid.
+Theorem op_id_r_uniq 
+  :  forall x : E, (op_is_id_r x) -> x = 0.
+Proof Monoid.op_id_r_uniq op_monoid.
 
 (** Proves that the identity element is unique. *)
-Definition op_id_uniq
-  :  forall x : E, (op_is_id x) -> x = 0
-  := Monoid.op_id_uniq op_monoid.
+Theorem op_id_uniq
+  :  forall x : E, (op_is_id x) -> x = 0.
+Proof Monoid.op_id_uniq op_monoid.
 
 (** Proves the left introduction rule. *)
-Definition op_intro_l
-  :  forall x y z : E, x = y -> z + x = z + y
-  := Monoid.op_intro_l op_monoid.
+Theorem op_intro_l
+  :  forall x y z : E, x = y -> z + x = z + y.
+Proof Monoid.op_intro_l op_monoid.
 
 (** Proves the right introduction rule. *)
-Definition op_intro_r
-  :  forall x y z : E, x = y -> x + z = y + z
-  := Monoid.op_intro_r op_monoid.
+Theorem op_intro_r
+  :  forall x y z : E, x = y -> x + z = y + z.
+Proof Monoid.op_intro_r op_monoid.
 
 (**
   Accepts two group elements, x and y, and
@@ -176,26 +178,27 @@ Definition op_is_inv := Monoid.op_is_inv op_monoid.
   Proves that for every group element, x,
   its left and right inverses are equal.
 *)
-Definition op_inv_l_r_eq
-  :  forall x y : E, op_is_inv_l x y -> forall z : E, op_is_inv_r x z -> y = z
-  := Monoid.op_inv_l_r_eq op_monoid.
+Theorem op_inv_l_r_eq
+  :  forall x y : E, op_is_inv_l x y -> forall z : E, op_is_inv_r x z -> y = z.
+Proof Monoid.op_inv_l_r_eq op_monoid.
 
 (**
   Proves that the inverse relation is
   symmetrical.
 *)
-Definition op_inv_sym
-  :  forall x y : E, op_is_inv x y <-> op_is_inv y x
-  := Monoid.op_inv_sym op_monoid.
+Theorem op_inv_sym
+  :  forall x y : E, op_is_inv x y <-> op_is_inv y x.
+Proof Monoid.op_inv_sym op_monoid.
 
 (**
   Proves that every group element has an
   inverse.
 *)
-Definition op_inv_ex
-  :  forall x : E, exists y : E, op_is_inv x y
-  := fun x : E
-       => ex_ind
+Theorem op_inv_ex
+  :  forall x : E, exists y : E, op_is_inv x y.
+Proof
+  fun x : E
+    => ex_ind
             (fun y H
               => ex_ind
                    (fun z H0
@@ -212,48 +215,53 @@ Definition op_inv_ex
             (op_inv_l_ex x).
 
 (** Proves the left cancellation rule. *)
-Definition op_cancel_l
-  :  forall x y z : E, z + x = z + y -> x = y
-  := fun x y z H 
-       => Monoid.op_cancel_l op_monoid x y z (op_inv_l_ex z) H.
+Theorem op_cancel_l
+  :  forall x y z : E, z + x = z + y -> x = y.
+Proof
+  fun x y z H 
+    => Monoid.op_cancel_l op_monoid x y z (op_inv_l_ex z) H.
 
 (** Proves the right cancellation rule. *)
-Definition op_cancel_r
-  :  forall x y z : E, x + z = y + z -> x = y
-  := fun x y z
-       => Monoid.op_cancel_r op_monoid x y z (op_inv_r_ex z).
+Theorem op_cancel_r
+  :  forall x y z : E, x + z = y + z -> x = y.
+Proof
+  fun x y z
+    => Monoid.op_cancel_r op_monoid x y z (op_inv_r_ex z).
 
 (**
   Proves that an element's left inverse
   is unique.
 *)
-Definition op_inv_l_uniq
-  :  forall x y z : E, op_is_inv_l x y -> op_is_inv_l x z -> z = y
-  := fun x
-       => Monoid.op_inv_l_uniq op_monoid x (op_inv_r_ex x).
+Theorem op_inv_l_uniq
+  :  forall x y z : E, op_is_inv_l x y -> op_is_inv_l x z -> z = y.
+Proof
+  fun x
+    => Monoid.op_inv_l_uniq op_monoid x (op_inv_r_ex x).
 
 (**
   Proves that an element's right inverse
   is unique.
 *)
-Definition op_inv_r_uniq
-  :  forall x y z : E, op_is_inv_r x y -> op_is_inv_r x z -> z = y
-  := fun x
-       => Monoid.op_inv_r_uniq op_monoid x (op_inv_l_ex x).
+Theorem op_inv_r_uniq
+  :  forall x y z : E, op_is_inv_r x y -> op_is_inv_r x z -> z = y.
+Proof
+  fun x
+    => Monoid.op_inv_r_uniq op_monoid x (op_inv_l_ex x).
 
 (** Proves that an element's inverse is unique. *)
-Definition op_inv_uniq
-  :  forall x y z : E, op_is_inv x y -> op_is_inv x z -> z = y
-  := Monoid.op_inv_uniq op_monoid.
+Theorem op_inv_uniq
+  :  forall x y z : E, op_is_inv x y -> op_is_inv x z -> z = y.
+Proof Monoid.op_inv_uniq op_monoid.
 
 (**
   Proves explicitly that every element has a
   unique inverse.
 *)
-Definition op_inv_uniq_ex
-  :  forall x : E, exists! y : E, op_is_inv x y
-  := fun x
-       => ex_ind
+Theorem op_inv_uniq_ex
+  :  forall x : E, exists! y : E, op_is_inv x y.
+Proof
+  fun x
+    => ex_ind
             (fun y (H : op_is_inv x y)
               => ex_intro 
                    (fun y => op_is_inv x y /\ forall z, op_is_inv x z -> y = z)
@@ -274,9 +282,11 @@ Definition op_neg
 Notation "{-}" := (op_neg) : group_scope.
 
 (** Asserts that the negation returns the inverse of its argument *)
-Definition op_neg_def
-  :  forall x : E, op_is_inv x ({-} x)
-  := fun x => Monoid.op_neg_def op_monoid x (op_inv_ex x).
+Theorem op_neg_def
+  :  forall x : E, op_is_inv x ({-} x).
+Proof
+  fun x
+    => Monoid.op_neg_def op_monoid x (op_inv_ex x).
 
 (** Proves that negation is one-to-one *)
 (** 0 = 0
@@ -285,42 +295,48 @@ Definition op_neg_def
    x + -x = y + -x
         x = y
 *)
-Definition op_neg_inj
-  :  is_injective E E op_neg
-  := fun x y
-       => Monoid.op_neg_inj op_monoid x (op_inv_ex x) y (op_inv_ex y).
+Theorem op_neg_inj
+  :  is_injective E E op_neg.
+Proof
+  fun x y
+    => Monoid.op_neg_inj op_monoid x (op_inv_ex x) y (op_inv_ex y).
 
 (** Proves the cancellation property for negation. *)
-Definition op_cancel_neg
-  :  forall x : E, {-} ({-} x) = x
-  := fun x
-       => Monoid.op_cancel_neg_gen op_monoid x (op_inv_ex x) (op_inv_ex ({-} x)).
+Theorem op_cancel_neg
+  :  forall x : E, {-} ({-} x) = x.
+Proof
+  fun x
+    => Monoid.op_cancel_neg_gen op_monoid x (op_inv_ex x) (op_inv_ex ({-} x)).
 
 (** Proves that negation is surjective - onto *)
-Definition op_neg_onto
-  :  is_onto E E {-}
-  := fun x => ex_intro (fun y => {-} y = x) ({-} x) (op_cancel_neg x).
+Theorem op_neg_onto
+  :  is_onto E E {-}.
+Proof
+  fun x => ex_intro (fun y => {-} y = x) ({-} x) (op_cancel_neg x).
 
 (** Proves that negation is bijective. *)
-Definition op_neg_bijective
-  :  is_bijective E E {-}
-  := conj op_neg_inj op_neg_onto.
+Theorem op_neg_bijective
+  :  is_bijective E E {-}.
+Proof
+  conj op_neg_inj op_neg_onto.
 
 (** Proves that neg x = y -> neg y = x *)
-Definition op_neg_rev
-  :  forall x y : E, {-} x = y -> {-} y = x
-  := fun x y H
-       => eq_sym
+Theorem op_neg_rev
+  :  forall x y : E, {-} x = y -> {-} y = x.
+Proof
+  fun x y H
+    => eq_sym
             (f_equal {-} H
              || a = {-} y @a by <- op_cancel_neg x).
 
 (**
   Proves that the left inverse of x + y is -y + -x.
 *)
-Definition op_neg_distrib_inv_l
-  :  forall x y : E, op_is_inv_l (x + y) ({-} y + {-} x)
-  := fun x y
-       => ((proj2 (op_neg_def ({-} y)))
+Theorem op_neg_distrib_inv_l
+  :  forall x y : E, op_is_inv_l (x + y) ({-} y + {-} x).
+Proof
+  fun x y
+    => ((proj2 (op_neg_def ({-} y)))
             || {-} y + a = 0                 @a by <- op_cancel_neg y
             || {-} y + a = 0                 @a by op_id_l y
             || {-} y + (a + y) = 0           @a by proj2 (op_neg_def ({-} x))
@@ -331,10 +347,11 @@ Definition op_neg_distrib_inv_l
 (**
   Proves that the right inverse of x + y is -y + -x.
 *)
-Definition op_neg_distrib_inv_r
-  :  forall x y : E, op_is_inv_r (x + y) ({-} y + {-} x)
-  := fun x y
-       => ((proj2 (op_neg_def x))
+Theorem op_neg_distrib_inv_r
+  :  forall x y : E, op_is_inv_r (x + y) ({-} y + {-} x).
+Proof
+  fun x y
+    => ((proj2 (op_neg_def x))
             || x + a = 0           @a by op_id_l ({-} x)
             || x + (a + {-} x) = 0 @a by proj2 (op_neg_def y)
             || x + a = 0           @a by op_is_assoc y ({-} y) ({-} x)
@@ -343,10 +360,11 @@ Definition op_neg_distrib_inv_r
 (**
   Proves that the inverse of x + y is -y + -x.
 *)
-Definition op_neg_distrib_inv
-  :  forall x y : E, op_is_inv (x + y) ({-} y + {-} x)
-  := fun x y
-       => conj
+Theorem op_neg_distrib_inv
+  :  forall x y : E, op_is_inv (x + y) ({-} y + {-} x).
+Proof
+  fun x y
+    => conj
             (op_neg_distrib_inv_l x y)
             (op_neg_distrib_inv_r x y).
 
@@ -354,10 +372,11 @@ Definition op_neg_distrib_inv
   Proves that negation is distributive: i.e.
   -(x + y) = -y + -x.
 *)
-Definition op_neg_distrib
-  :  forall x y : E, {-} (x + y) = {-} y + {-} x
-  := fun x y
-       => ex_ind
+Theorem op_neg_distrib
+  :  forall x y : E, {-} (x + y) = {-} y + {-} x.
+Proof
+  fun x y
+    => ex_ind
             (fun z (H : unique (op_is_inv (x + y)) z)
               => let H0
                    :  z = {-} (x + y)
@@ -375,5 +394,11 @@ Definition op_neg_distrib
 End Theorems.
 
 End Group.
+
+Notation "0" := (Group.E_0) : group_scope.
+
+Notation "x + y" := (Group.op x y) (at level 50, left associativity) : group_scope.
+
+Notation "{+}" := (Group.op) : group_scope.
 
 Notation "{-}" := (Group.op_neg _) : group_scope.
